Veritas.BinTreePtr.fsti
@@ -8,9 +8,19 @@ open Veritas.BinTree
  *)
 type ptrfn = (n:bin_tree_node) -> (c:bin_tree_dir) -> option (d:bin_tree_node{is_desc d (child c n)})
 
+(* does n point to some node along direction c *)
+let points_to_some (pf:ptrfn) (n:bin_tree_node) (c:bin_tree_dir): bool = 
+  Some? (pf n c)
+
+(* if n points to n' along c, return n' *)
+let pointed_node (pf:ptrfn) (n:bin_tree_node) (c:bin_tree_dir {points_to_some pf n c}): bin_tree_node = 
+  Some?.v (pf n c)
+
+(* does a point to d *)
 let points_to (pf: ptrfn) (d: bin_tree_node) (a: bin_tree_node{is_proper_desc d a}): bool = 
   let c = desc_dir d a in
-  Some? (pf a c) && d = Some?.v (pf a c) 
+  points_to_some pf a c && 
+  d = pointed_node pf a c 
 
 (* Is d reachable from a following pf pointers *)
 val reachable (pf: ptrfn) (d a: bin_tree_node): Tot bool
@@ -54,3 +64,42 @@ val lemma_non_reachable_desc_of_none (pf: ptrfn)
                                      (a:bin_tree_node{is_proper_desc d a /\ 
                                                       None? (pf a (desc_dir d a))}):
   Lemma (not (reachable pf d a))
+
+(* Extend the pointer functio with a new points_to edge *)
+let extend_ptrfn (pf:ptrfn) 
+                 (d:bin_tree_node) 
+                 (a:bin_tree_node{is_proper_desc d a /\
+                                  not (points_to_some pf a (desc_dir d a))}): ptrfn = 
+  let c = desc_dir d a in
+  fun n' c' -> if n' = a && c' = c then Some d else pf n' c'
+
+(* extension does not reduce reachability *)
+val lemma_extend_reachable (pf:ptrfn) 
+                           (d1:bin_tree_node) 
+                           (a1:bin_tree_node{is_proper_desc d1 a1 /\ 
+                                            not (points_to_some pf a1 (desc_dir d1 a1))})
+                           (d: bin_tree_node)
+                           (a: bin_tree_node):
+  Lemma (requires (reachable pf d a))
+        (ensures (reachable (extend_ptrfn pf d1 a1) d a))
+
+(* Extend the pointer function by cutting a pointer *)
+let extendcut_ptrfn (pf:ptrfn)
+                    (d:bin_tree_node)
+                    (a:bin_tree_node{is_proper_desc d a /\ 
+                                     points_to_some pf a (desc_dir d a) /\
+                                     is_proper_desc (pointed_node pf a (desc_dir d a)) d}): ptrfn = 
+   let c1 = desc_dir d a in
+   let d' = pointed_node pf a c1 in
+   let c2 = desc_dir d' d in
+   fun n' c' -> if n' = a && c' = c1 then Some d 
+              else if n' = d && c' = c2 then Some d' 
+              else pf n' c'
+
+let feq_ptrfn (pf1: ptrfn) (pf2: ptrfn) = 
+  forall n. forall c. {:pattern (pf1 n c) \/ (pf2 n c)} pf1 n c == pf2 n c
+
+val lemma_reachable_feq (pf1: ptrfn) (pf2: ptrfn) (d: bin_tree_node) (a: bin_tree_node):
+  Lemma (requires (feq_ptrfn pf1 pf2))
+        (ensures (reachable pf1 d a = reachable pf2 d a))
+                   
